WIP interp_total_function

src/Syntax.v
@@ -380,12 +380,15 @@ Section syntax.
 
 
   (* TODO free_evars, free_svars *)
-  Class EBinder (ebinder : Pattern -> Pattern) :=
+Class EBinder (ebinder : Pattern -> Pattern)
+      (fevo: db_index -> evar -> Pattern -> Pattern )
+      (fsvo: db_index -> svar -> Pattern -> Pattern ) :=
     {
       ebinder_evar_open :
-        forall k n ϕ, evar_open k n (ebinder ϕ) = ebinder (evar_open (k + 1) n ϕ) ;
+        forall k n ϕ, evar_open k n (ebinder ϕ) = fevo k n ϕ ;
+                        (*ebinder (evar_open (k + 1) n ϕ) ;*)
       ebinder_svar_open :
-        forall k n ϕ, svar_open k n (ebinder ϕ) = ebinder (svar_open k n ϕ) ;
+        forall k n ϕ, svar_open k n (ebinder ϕ) = fsvo k n ϕ ; (*ebinder (svo a) (svar_open k n ϕ) ;*)
     }.
 
   Class SBinder (sbinder : Pattern -> Pattern) :=
@@ -440,7 +443,7 @@ Section syntax.
   
 
   #[global]
-  Instance EBinder_exists : EBinder patt_exists :=
+  Instance EBinder_exists : EBinder patt_exists _ _ :=
     {|
        ebinder_evar_open := evar_open_exists ;
        ebinder_svar_open := svar_open_exists ;
@@ -1589,7 +1592,7 @@ Section syntax.
     |}.
 
   #[global]
-  Instance EBinder_forall : EBinder patt_forall :=
+  Instance EBinder_forall : EBinder patt_forall _ _ :=
     {|
        ebinder_evar_open := evar_open_forall ;
        ebinder_svar_open := svar_open_forall ;
@@ -2138,7 +2141,7 @@ Section syntax.
     done.
   Qed.
 
-  Hint Resolve evar_is_fresh_in_app_l : core.
+  (*Hint Resolve evar_is_fresh_in_app_l : core.*)
 
   Lemma evar_is_fresh_in_app_r x ϕ₁ ϕ₂ :
     evar_is_fresh_in x (patt_app ϕ₁ ϕ₂) -> evar_is_fresh_in x ϕ₂.
@@ -2148,7 +2151,7 @@ Section syntax.
     done.
   Qed.
 
-  Hint Resolve evar_is_fresh_in_app_r : core.
+  (*Hint Resolve evar_is_fresh_in_app_r : core.*)
 
   Lemma evar_is_fresh_in_imp_l x ϕ₁ ϕ₂ :
     evar_is_fresh_in x (patt_imp ϕ₁ ϕ₂) -> evar_is_fresh_in x ϕ₁.
@@ -2158,7 +2161,7 @@ Section syntax.
     done.
   Qed.
 
-  Hint Resolve evar_is_fresh_in_imp_l : core.
+  (*Hint Resolve evar_is_fresh_in_imp_l : core.*)
 
   Lemma evar_is_fresh_in_imp_r x ϕ₁ ϕ₂ :
     evar_is_fresh_in x (patt_imp ϕ₁ ϕ₂) -> evar_is_fresh_in x ϕ₂.
@@ -2168,7 +2171,7 @@ Section syntax.
     done.
   Qed.
 
-  Hint Resolve evar_is_fresh_in_imp_r : core.
+  (*Hint Resolve evar_is_fresh_in_imp_r : core.*)
 
   Lemma evar_is_fresh_in_exists x ϕ :
     evar_is_fresh_in x (patt_exists ϕ) -> evar_is_fresh_in x ϕ.
@@ -2176,7 +2179,7 @@ Section syntax.
     unfold evar_is_fresh_in. simpl. done.
   Qed.
 
-  Hint Resolve evar_is_fresh_in_exists : core.
+  (*Hint Resolve evar_is_fresh_in_exists : core.*)
 
   Lemma evar_is_fresh_in_mu x ϕ :
     evar_is_fresh_in x (patt_mu ϕ) -> evar_is_fresh_in x ϕ.
@@ -2184,7 +2187,7 @@ Section syntax.
     unfold evar_is_fresh_in. simpl. done.
   Qed.
 
-  Hint Resolve evar_is_fresh_in_mu : core.
+  (*Hint Resolve evar_is_fresh_in_mu : core.*)
 
   (**)
   Lemma svar_is_fresh_in_app_l x ϕ₁ ϕ₂ :
